spill_live: only 2 subcases still missing

theories/Spilling/Soundness.v
@@ -1,164 +1,9 @@
 Require Import List Map Env AllInRel Exp AppExpFree.
 Require Import IL Annotation InRel AutoIndTac Liveness LabelsDefined.
-Require Import SimI Spilling.
+Require Import SimI Spilling DoSpill.
 
 Set Implicit Arguments.
 
-
-Fixpoint write_spills (slot: var->var) (xs:list var) (s:stmt) : stmt :=
-match xs with
-| nil => s
-| x::xs => stmtLet (slot x) (Operation (Var x)) (write_spills slot xs s)
-end.
-
-Fixpoint write_loads (slot: var-> var) (xs:list var) (s:stmt) : stmt :=
-match xs with
-| nil => s
-| x::xs => stmtLet x (Operation (Var (slot x))) (write_loads slot xs s)
-end.
-
-
-Fixpoint do_spill
-(slot: var -> var)
-(s:stmt)
-(sl:ann (set var * set var * option (list (set var * set var)))) : stmt :=
-
-let Sp := fst (fst (getAnn sl)) in
-let L  := snd (fst (getAnn sl)) in
-
-write_spills slot (elements Sp)
-  (write_loads slot (elements L)
-
-    (match s,sl with
-     | stmtLet x e s, ann1 _ sl_s
-       => stmtLet x e (do_spill slot s sl_s)
-     | stmtIf e s t, ann2 _ sl_s sl_t
-       => stmtIf e (do_spill slot s sl_s) (do_spill slot t sl_t)
-     | stmtFun F t, annF _ sl_F sl_t
-       => stmtFun
-            ((fun Zs sl_s => (fst Zs (* todo: really? I think it's fine *)
-                                    , do_spill slot (snd Zs) sl_s)) ⊜ F sl_F)
-            (do_spill slot t sl_t)
-
-     | _,_
-       => s
-     end))
-.
-
-Fixpoint test
-         (s : set var)
-         (n : nat)
-         {struct n}
-  : set var
-  :=
-    match n with
-    | 0 => s
-    | S n => test (of_list (tl (elements s))) n
-    end.
-
-
-Fixpoint do_spill'
-         (slot : var -> var)
-         (s : stmt)
-         (sl : ann (set var * set var * option(list(set var * set var))))
-         {struct s}
-  : stmt :=
-
-
-
-  let Sp := fst (fst (getAnn sl)) in
-  let L  := snd (fst (getAnn sl)) in
-  let rm := snd (getAnn sl) in
-
-(fix f sl n {struct n} :=
-  match n with
-    | 0 =>
-     match s,sl with
-     | stmtLet x e s, ann1 _ sl_s
-       => stmtLet x e (do_spill' slot s sl_s)
-     | stmtIf e s t, ann2 _ sl_s sl_t
-       => stmtIf e (do_spill' slot s sl_s) (do_spill' slot t sl_t)
-     | stmtFun F t, annF _ sl_F sl_t
-       => stmtFun
-            ((fun Zs sl_s => (fst Zs (* todo: really? I think it's fine *)
-                                    , do_spill' slot (snd Zs) sl_s)) ⊜ F sl_F)
-                           (do_spill' slot t sl_t)
-
-     | _,_
-       => s
-     end
-    | S n =>
-
-  if
-    [cardinal Sp = 0]
-  then
-    if
-      [cardinal L = 0]
-    then
-     match s,sl with
-     | stmtLet x e s, ann1 _ sl_s
-       => stmtLet x e (do_spill' slot s sl_s)
-     | stmtIf e s t, ann2 _ sl_s sl_t
-       => stmtIf e (do_spill' slot s sl_s) (do_spill' slot t sl_t)
-     | stmtFun F t, annF _ sl_F sl_t
-       => stmtFun
-            ((fun Zs sl_s => (fst Zs (* todo: really? I think it's fine *)
-                                    , do_spill' slot (snd Zs) sl_s)) ⊜ F sl_F)
-                           (do_spill' slot t sl_t)
-
-     | _,_
-       => s
-     end
-
-    else
-      let x := hd 0 (elements L) in
-      let L':= of_list (tl (elements L)) in
-      stmtLet x (Operation (Var (slot x))) (f (setTopAnn sl (Sp,L',rm)) n)
-
-  else
-    let x  := hd 0 (elements Sp) in
-    let Sp':= of_list (tl (elements Sp)) in
-    stmtLet (slot x) (Operation (Var x)) (f (setTopAnn sl (Sp',L,rm)) n)
-  end
-) sl (cardinal Sp + cardinal L)
-.
-
-
-
-Lemma do_spill_empty
-      (slot : var -> var)
-      (s : stmt)
-      (sl : ann (set var * set var * option (list (set var * set var))))
-  :
-    Empty (fst (fst (getAnn sl)))
-    -> Empty (snd (fst (getAnn sl)))
-    -> do_spill' slot s sl
-      =
-
-      match s,sl with
-     | stmtLet x e s, ann1 _ sl_s
-       => stmtLet x e (do_spill' slot s sl_s)
-     | stmtIf e s t, ann2 _ sl_s sl_t
-       => stmtIf e (do_spill' slot s sl_s) (do_spill' slot t sl_t)
-     | stmtFun F t, annF _ sl_F sl_t
-       => stmtFun
-            ((fun Zs sl_s => (fst Zs, do_spill' slot (snd Zs) sl_s)) ⊜ F sl_F)
-            (do_spill' slot t sl_t)
-
-     | _,_
-       => s
-      end.
-Proof.
-  intros Empty_Sp Empty_L.
-  remember (fst (fst (getAnn sl))) as Sp.
-  remember (snd (fst (getAnn sl))) as L.
-  assert (cardinal Sp = 0) as zero_Sp.
-  { apply cardinal_Empty. eauto. }
-  assert (cardinal L = 0) as zero_L.
-  { apply cardinal_Empty. eauto. }
-  induction sl, s; simpl in *; rewrite <- HeqSp; rewrite <- HeqL;
-    simpl; rewrite zero_Sp; rewrite zero_L; simpl; eauto.
-Qed.
 
 Definition discard_sl := mapAnn (fun (a : (* = mapAnn ? snd *)
       set var * set var * option (list (set var * set var)))
@@ -179,15 +24,6 @@ mapAnn (fun (a : set var * set var * option (list (set var * set var)))
               => Some (slot_merge slot rms)
            end).
 
-Lemma discard_merge_sl_1
-      (slot : var -> var)
-      (Sp L : set var)
-      (sl : ann (set var * set var * option ( list (set var * set var))))
-  :
-    discard_merge_sl slot (ann1 (Sp,L,None) sl) = ann1 None (discard_merge_sl slot sl).
-Proof.
-  eauto.
-Qed.
 
 Lemma discard_merge_sl_step
       (slot : var -> var)
@@ -218,382 +54,167 @@ Lemma discard_merge_sl_step
     end.
 Proof.
   induction sl; destruct a as [spl rm]; induction rm;
-    unfold discard_merge_sl; fold discard_merge_sl; simpl; admit.
-(* trivial! but how to kill the stupid let (_,_) ?? *)
-Admitted.
-
-
-
-(*
-Lemma discard_merge_sl_set_invariant
-      (slot : var -> var)
-      (a a' : ann (set var * set var * option(list(set var * set var))))
-  :
-    a === a'
-      -> discard_merge_sl slot a === discard_merge_sl slot a'.
-Proof.
-  intro aEq.
-  induction a, a'; try isabsurd.
-  - econstructor.
-
-    destruct a as [[Sp L] [rm |]];
-      destruct a0 as [[Sp0 L0] [rm0|]];
-      inversion_clear aEq; inversion_clear H; inversion_clear H1.
-    + econstructor. simpl. induction rm,rm0; try isabsurd.
-      * econstructor.
-      * econstructor.
-        -- admit.
-        -- admit.
-    + econstructor.
-  - econstructor.
-    + destruct a as [[Sp L] [rm |]];
-        destruct a1 as [[Sp1 L1] [rm1 |]];
-        inversion_clear aEq; inversion_clear H; inversion_clear H1; admit.
-    + admit.
-  - econstructor.
-    + destruct a as [[Sp L] [rm |]];
-        destruct a1 as [[Sp1 L1] [rm1 |]];
-        inversion_clear aEq; inversion_clear H; inversion_clear H1; admit.
-    + admit.
-    + admit.
-  - admit.
-Admitted.
-*)
-
-Lemma ann_R_seteq
-      (X : Type) `{OrderedType X}
-      (a b : ann X)
-  :
-    a === b
-    -> ann_R _eq a b.
-Proof.
-  intros eq_ab.
-  induction a,b ; try isabsurd; inversion eq_ab.
-  * apply annLt0. eauto.
-      * apply annLt1; eauto.
-      * apply annLt2; eauto.
-      * apply annLtF; eauto.
+    unfold discard_merge_sl; fold discard_merge_sl; simpl; destruct spl;
+      reflexivity.
 Qed.
 
-Lemma ann_seteq_0
-      (X : Type) `{OrderedType X}
-      (x x' : X)
-  :
-    x === x'
-    -> ann0 x === ann0 x'.
-Proof.
-  intros eq_x.
-  apply ann_R_Equivalence.
-  - apply OT_Equivalence.
-  - econstructor. eauto.
-Qed.
-
-
-
-
-Lemma ann_seteq_1
-      (X : Type) `{OrderedType X}
-      (x x' : X)
-      (a b : ann X)
-  :
-    x === x'
-    -> a === b
-    -> ann1 x a === ann1 x' b.
-Proof.
-  intros eq_x eq_ab.
-  apply ann_R_Equivalence.
-  - apply OT_Equivalence.
-  - econstructor.
-    + eauto.
-    + apply ann_R_seteq. eauto.
-Qed.
-
-Lemma ann_seteq_2
-      (X : Type) `{OrderedType X}
-      (x x' : X)
-      (a a' b b': ann X)
-  :
-    x === x'
-    -> a === a'
-    -> b === b'
-    -> ann2 x a b === ann2 x' a' b'.
-Proof.
-  intros eq_x eq_a eq_b.
-  apply ann_R_Equivalence.
-  - apply OT_Equivalence.
-  - econstructor.
-    + eauto.
-    + apply ann_R_seteq. eauto.
-    + apply ann_R_seteq. eauto.
-Qed.
-
-
-Lemma ann_seteq_F
-      (X : Type) `{OrderedType X}
-      (x x' : X)
-      (a a': ann X)
-      (F F': list (ann X))
-  :
-    x === x'
-    -> a === a'
-    -> F === F'
-    -> annF x F a === annF x' F' a'.
-Proof.
-  intros eq_x eq_a eq_F.
-  apply ann_R_Equivalence.
-  - apply OT_Equivalence.
-  - econstructor.
-    + eauto.
-    + revert dependent F'. revert F. induction F.
-      * induction F'.
-        -- eauto.
-        -- isabsurd.
-      * destruct F'.
-        -- isabsurd.
-        -- intros. simpl. f_equal. apply IHF.
-           inversion_clear eq_F.
-           apply H0.
-    + intros n a0 b get_a0 get_b.
-      enough (a0 === b) as eq_ab.
-      * rewrite eq_ab.
-        apply ann_R_refl.
-      * eapply get_PIR2 with (L:=F') (L':=F) (n:=n).
-        -- symmetry in eq_F. eauto.
-        -- eauto.
-        -- eauto.
-    + apply ann_R_seteq. eauto.
-Qed.
-
-
-
-Lemma ann_seteq_s_t_1
-      (s s' t t' : set var)
-      (rm : option(list(set var * set var)))
-      (sl : ann (set var * set var * option(list(set var * set var))))
-  :
-    s === s'
-    -> t === t'
-        -> ann1 (s,t,rm) sl === ann1 (s',t',rm) sl.
-Proof.
-  intros eq_s eq_t.
-  apply ann_R_Equivalence.
-      - apply OT_Equivalence.
-      - econstructor.
-        + econstructor.
-          * econstructor; eauto.
-          * eauto.
-        + eauto.
-Qed.
-
-
-Fixpoint add_nones
-         (n : nat)
-         (b : ann (set var * set var * option(list( set var * set var))))
-  : ann (set var * set var * option (list ( set var * set var)))
-      :=
-        match n with
-        |   0 => b
-        | S(n)=> ann1 (∅,∅,None) (add_nones n b)
-        end.
-
-
-
-
-Fixpoint do_spill_rm
-(slot : var -> var)
-(sl: ann (set var * set var * option (list (set var * set var ))))
-: ann (set var * set var * option (list (set var * set var)))
-:=
-match sl with
-| ann0 (Sp,L,rm)           => add_nones (cardinal Sp + cardinal L)
-                                         sl
-| ann1 (Sp,L,rm) sl_s      => add_nones (cardinal Sp + cardinal L)
-                                        (ann1 (Sp,L,rm) (do_spill_rm slot sl_s))
-| ann2 (Sp,L,rm) sl_s sl_t => add_nones (cardinal Sp + cardinal L)
-                                        (ann2 (Sp,L,rm) (do_spill_rm slot sl_s)
-                                                        (do_spill_rm slot sl_t))
-| annF (Sp,L,rm) sl_F sl_t => add_nones (cardinal Sp + cardinal L)
-                                  (annF (Sp,L,rm) (do_spill_rm slot ⊝ sl_F)
-                                                  (do_spill_rm slot sl_t))
-end.
 
 (*
 Fixpoint do_spill_rm
 (slot : var -> var)
-(sl: ann (set var * set var * option (list (set var * set var ))))
+(sl0: ann (set var * set var * option (list (set var * set var ))))
+{struct sl0}
 : ann (set var * set var * option (list (set var * set var)))
   :=
-    add_nones (cardinal Sp + cardinal L)
+    let Sp0 := fst (fst (getAnn sl0)) in
+    let L0  := snd (fst (getAnn sl0)) in
+    (fix f sl n {struct n} :=
+      let Sp := fst (fst (getAnn sl)) in
+      let L  := snd (fst (getAnn sl)) in
+      let rm := snd (getAnn sl) in
+      match n with
+      | 0 =>
+        match sl0 with
+        | ann0 (Sp,L,rm)
+          => sl
+        | ann1 (Sp,L,rm) sl_s
+          => ann1 (Sp,L,rm) (do_spill_rm slot sl_s)
+        | ann2 (Sp,L,rm) sl_s sl_t
+          => ann2 (Sp,L,rm) (do_spill_rm slot sl_s)
+                            (do_spill_rm slot sl_t)
+        | annF (Sp,L,rm) sl_F sl_t
+          => annF (Sp,L,rm) (do_spill_rm slot ⊝ sl_F)
+                            (do_spill_rm slot    sl_t)
+        end
+      | S n =>
+        if [cardinal Sp = 0]
+        then
+          if [cardinal L = 0]
+          then
+            match sl0 with
+            | ann0 (Sp,L,rm)
+              => sl
+            | ann1 (Sp,L,rm) sl_s
+              => ann1 (Sp,L,rm) (do_spill_rm slot sl_s)
+            | ann2 (Sp,L,rm) sl_s sl_t
+              => ann2 (Sp,L,rm) (do_spill_rm slot sl_s)
+                                (do_spill_rm slot sl_t)
+            | annF (Sp,L,rm) sl_F sl_t
+              => annF (Sp,L,rm) (do_spill_rm slot ⊝ sl_F)
+                                (do_spill_rm slot    sl_t)
+            end
+          else
+            let L' := of_list (tl (elements L)) in
+            ann1 (∅,∅,None) (f (setTopAnn sl (Sp,L',rm)) n)
+        else
+          let Sp' := of_list (tl (elements Sp)) in
+          ann1 (∅,∅,None) (f (setTopAnn sl (Sp',L,rm)) n)
+      end
+    ) sl0 (cardinal Sp0 + cardinal L0)
+.
 
-match sl with
-| ann0 (Sp,L,rm)           => sl
-| ann1 (Sp,L,rm) sl_s      => ann1 (Sp,L,rm) (do_spill_rm slot sl_s)
-| ann2 (Sp,L,rm) sl_s sl_t => ann2 (Sp,L,rm) (do_spill_rm slot sl_s)
-                                             (do_spill_rm slot sl_t)
-| annF (Sp,L,rm) sl_F sl_t => annF (Sp,L,rm) (do_spill_rm slot ⊝ sl_F)
-                                             (do_spill_rm slot sl_t)
-end.
 *)
-
-Lemma do_spill_rm_empty'
+(*
+Fixpoint do_spill_rm'
 (slot : var -> var)
-(sl : ann (set var * set var * option (list (set var * set var ))))
-(rm : option(list(set var * set var)))
-  : getAnn sl === (∅,∅,rm)
-    -> do_spill_rm slot sl ===
-     match sl with
-     | ann0 _ => ann0 (∅,∅,rm)
-     | ann1 _ sl_s => ann1 (∅,∅,rm) (do_spill_rm slot sl_s)
-     | ann2 _ sl_s sl_t => ann2 (∅,∅,rm) (do_spill_rm slot sl_s)
-                                         (do_spill_rm slot sl_t)
-     | annF _ sl_F sl_t => annF (∅,∅,rm) (do_spill_rm slot ⊝ sl_F)
-                                         (do_spill_rm slot sl_t)
-     end.
-Proof. (*
-intros emptySpL.
-induction sl; simpl in *. (*+TODO+*)
-- eauto.
-- rewrite empty_cardinal. simpl. eauto.
-- rewrite empty_cardinal. simpl. eauto.
-- rewrite empty_cardinal. simpl. eauto.
-Qed.
-        *)
-Admitted.
+(sl: ann (set var * set var * option (list (set var * set var ))))
+{struct sl}
+: ann (set var * set var * option (list (set var * set var)))
+  :=
+    let Sp := fst (fst (getAnn sl)) in
+    let L  := snd (fst (getAnn sl)) in
+    (fix f n {struct n} :=
+      match n with
+      | 0 =>
+        match sl with
+        | ann0 _
+          => sl
+        | ann1 a sl_s
+          => ann1 a (do_spill_rm' slot sl_s)
+        | ann2 a sl_s sl_t
+          => ann2 a (do_spill_rm' slot sl_s)
+                    (do_spill_rm' slot sl_t)
+        | annF a sl_F sl_t
+          => annF a (do_spill_rm' slot ⊝ sl_F)
+                    (do_spill_rm' slot   sl_t)
+        end
+      | S n =>
+        if [cardinal Sp + cardinal L = 0]
+        then
+          match sl with
+          | ann0 a
+            => sl
+          | ann1 a sl_s
+            => ann1 a (do_spill_rm' slot sl_s)
+          | ann2 a sl_s sl_t
+            => ann2 a (do_spill_rm' slot sl_s)
+                      (do_spill_rm' slot sl_t)
+          | annF a sl_F sl_t
+            => annF a (do_spill_rm' slot ⊝ sl_F)
+                      (do_spill_rm' slot    sl_t)
+          end
+        else
+          ann1 (∅,∅,None) (f n)
+      end
+    ) (cardinal Sp + cardinal L)
+.
+*)
+Function count
+         (sl : ann (set var * set var * option (list (set var * set var))))
+  := cardinal (fst (fst (getAnn sl))) + cardinal (snd (fst (getAnn sl))).
 
-Lemma do_spill_rm_empty
-(slot : var -> var)
-(sl : ann (set var * set var * option (list (set var * set var ))))
-(rm : option(list(set var * set var)))
-  : getAnn sl = (∅,∅,rm)
-    -> do_spill_rm slot sl =
-     match sl with
-     | ann0 _ => ann0 (∅,∅,rm)
-     | ann1 _ sl_s => ann1 (∅,∅,rm) (do_spill_rm slot sl_s)
-     | ann2 _ sl_s sl_t => ann2 (∅,∅,rm) (do_spill_rm slot sl_s)
-                                         (do_spill_rm slot sl_t)
-     | annF _ sl_F sl_t => annF (∅,∅,rm) (do_spill_rm slot ⊝ sl_F)
-                                         (do_spill_rm slot sl_t)
-     end.
-Proof.
-intros emptySpL.
-induction sl; simpl in *; rewrite emptySpL.
-- eauto.
-- rewrite empty_cardinal. simpl. eauto.
-- rewrite empty_cardinal. simpl. eauto.
-- rewrite empty_cardinal. simpl. eauto.
-Qed.
+Fixpoint do_spill_rm'
+         (slot : var -> var)
+         (n : nat)
+         (sl: ann (set var * set var * option (list (set var * set var ))))
+         {struct sl}
+  : ann (set var * set var * option (list (set var * set var)))
+  :=
+    let rm := snd (getAnn sl) in
+    (fix add_nones n
+        :=
+    match n with
+    | 0 =>
+        match sl with
+        | ann0 a => sl
+        | ann1 a sl_s
+          => ann1 a (do_spill_rm' slot (count sl_s) sl_s)
+        | ann2 a sl_s sl_t
+          => ann2 a (do_spill_rm' slot (count sl_s) sl_s)
+                    (do_spill_rm' slot (count sl_t) sl_t)
+        | annF a sl_F sl_t
+          => annF a ((fun sl_s => do_spill_rm' slot (count sl_s) sl_s) ⊝ sl_F)
+                    (do_spill_rm' slot (count   sl_t) sl_t)
+        end
+    | S n =>
+        ann1 (∅,∅,None) (add_nones n)
+    end) n
+.
 
 
-Lemma do_spill_rm_empty''
-(slot : var -> var)
-(sl : ann (set var * set var * option (list (set var * set var ))))
-  : Empty (fst (fst (getAnn sl)))
-    -> Empty (snd (fst (getAnn sl)))
-    -> do_spill_rm slot sl =
-     match sl with
-     | ann0 (Sp,L,rm) => ann0 (Sp,L,rm)
-     | ann1 (Sp,L,rm) sl_s => ann1 (Sp,L,rm) (do_spill_rm slot sl_s)
-     | ann2 (Sp,L,rm) sl_s sl_t => ann2 (Sp,L,rm) (do_spill_rm slot sl_s)
-                                         (do_spill_rm slot sl_t)
-     | annF (Sp,L,rm) sl_F sl_t => annF (Sp,L,rm) (do_spill_rm slot ⊝ sl_F)
-                                         (do_spill_rm slot sl_t)
-     end.
-Proof.
 
-intros Sp_Empty L_Empty.
-induction sl; destruct a as [[Sp L] rm']; simpl in *;
-  apply cardinal_Empty in Sp_Empty; apply cardinal_Empty in L_Empty;
-  rewrite Sp_Empty; rewrite L_Empty; simpl; eauto.
-Qed.
+Definition do_spill_rm
+           (slot : var -> var)
+           (sl : ann (set var * set var * option (list (set var * set var))))
+  := do_spill_rm' slot (count sl) sl.
+
+
 
 Lemma do_spill_rm_s
       (slot : var -> var)
       (sl : ann (set var * set var * option (list (set var * set var))))
       (n : nat)
   :
-    cardinal (fst (fst (getAnn sl))) + cardinal (snd (fst (getAnn sl))) = S n
-    -> do_spill_rm slot sl
-      = ann1 (∅,∅,None)
-             (add_nones n (
-     match sl with
-     | ann0 (Sp,L,rm) => ann0 (Sp,L,rm)
-     | ann1 (Sp,L,rm) sl_s => ann1 (Sp,L,rm) (do_spill_rm slot sl_s)
-     | ann2 (Sp,L,rm) sl_s sl_t => ann2 (Sp,L,rm) (do_spill_rm slot sl_s)
-                                         (do_spill_rm slot sl_t)
-     | annF (Sp,L,rm) sl_F sl_t => annF (Sp,L,rm) (do_spill_rm slot ⊝ sl_F)
-                                         (do_spill_rm slot sl_t)
-     end)).
-Proof.
-  intros card_s.
-  induction sl; destruct a as [[Sp L] rm']; simpl in *; rewrite card_s; simpl; eauto.
-Qed.
-
-
-
-Lemma do_spill_Sp
-      (slot : var -> var)
-      (s : stmt)
-      (sl : ann (set var * set var * option (list (set var * set var))))
-  :
-    let Sp := fst (fst (getAnn sl)) in
-    let L  := snd (fst (getAnn sl)) in
-    let x  := hd 0 (elements L) in
-    let Sp':= of_list (tl (elements Sp)) in
-    ~ Empty Sp
-    -> do_spill' slot s sl
-      = stmtLet (slot x)
-                (Operation (Var x))
-                (do_spill' slot s (setTopAnn sl (Sp',L,snd (getAnn sl))))
+    do_spill_rm' slot (S n) sl
+    = ann1 (∅,∅,None) (do_spill_rm' slot n sl)
 .
 Proof.
-  intros Sp0 L0 x Sp' NEmpty_Sp.
-  assert (~ cardinal Sp0 = 0) as Sp_nonzero.
-  { intro N. apply NEmpty_Sp. rewrite cardinal_Empty. eauto. }
-  subst Sp0...
-  subst L0...
-  destruct (getAnn sl) as [[Sp L] rm].
-  admit.
-Admitted.
-
-Lemma do_spill_L
-      (slot : var -> var)
-      (s : stmt)
-      (sl : ann (set var * set var * option (list (set var * set var))))
-:
-  let Sp := fst (fst (getAnn sl)) in
-  let L  := snd (fst (getAnn sl)) in
-  let x  := hd 0 (elements L) in
-  let L' := of_list (tl (elements L)) in
-  Empty Sp
-  -> ~ Empty L
-  -> do_spill' slot s sl
-    = stmtLet x
-              (Operation (Var (slot x)))
-              (do_spill' slot s (setTopAnn sl (Sp,L',snd (getAnn sl)))).
-Admitted.
-
-(*
-Corollary do_spill_rm_empty_1
-          (slot : var -> var)
-          (s t : set var)
-          (sl : ann (set var * set var * option(list(set var * set var))))
-  : s === ∅
-    -> t === ∅
-    -> do_spill_rm slot (ann1 (s,t,None) sl)
-                === ann1 (s,t,None) (do_spill_rm slot sl)
-.
-Proof. (*
-  intros s_eq t_eq.
-  assert (tada := ann_seteq_s_t_1 (*s ∅ t ∅*) None (do_spill_rm slot sl) s_eq t_eq).
-  rewrite tada.
-  rewrite do_spill_rm_empty'.
-  - eauto.
-  - simpl. apply injective_projections; simpl.
-    + apply injective_projections; simpl. eauto. rewrite s_eq. | rewrite t_eq]. eauto. reflexivity. eauto.
+  unfold do_spill_rm' at 1.
+  destruct sl;
+    simpl;
+    reflexivity.
 Qed.
-*)
-Admitted.
-*)
+
 
 Fixpoint spill_live
 (Lv : list (set var))
@@ -635,24 +256,6 @@ match s, rm with
 
 end.
 
-Lemma write_spills_empty
-(slot : var -> var)
-(s : stmt)
-: write_spills slot nil s = s.
-Proof.
-simpl.
-eauto.
-Qed.
-
-Lemma write_loads_empty
-(slot : var -> var)
-(s : stmt)
-: write_loads slot nil s = s.
-Proof.
-simpl.
-eauto.
-Qed.
-
 
 Lemma spill_live_G
       (Lv : list (set var))
@@ -668,6 +271,9 @@ Proof.
     cset_tac.
 Qed.
 
+
+
+(* move somewhere *)
 Lemma setTopAnn_setTopAnn
       (X : Type)
       (x x' : X)
@@ -678,6 +284,8 @@ Proof.
   induction a; simpl; eauto.
 Qed.
 
+
+(* TODO: move to DoSpill.v *)
 Lemma do_spill_empty_invariant
       (slot : var -> var)
       (s : stmt)
@@ -690,7 +298,7 @@ Lemma do_spill_empty_invariant
     -> Empty (snd (fst (getAnn sl)))
     -> Empty Sp'
     -> Empty L'
-    -> do_spill' slot s sl = do_spill' slot s sl'
+    -> do_spill slot s sl = do_spill slot s sl'
 .
 Proof.
   intros top_sl' Empty_Sp Empty_L Empty_Sp' Empty_L'.
@@ -702,9 +310,10 @@ Proof.
   unfold setTopAnn.
   induction sl; simpl; reflexivity.
 Qed.
-
+(*
 Lemma dms_dsr_empty_invariant
       (slot : var -> var)
+      (n n': nat)
       (Sp' L' : set var)
       (rm : option (list (set var * set var)))
       (sl sl' : ann (set var * set var * option (list (set var * set var))))
@@ -714,181 +323,304 @@ Lemma dms_dsr_empty_invariant
   -> Empty (snd (fst (getAnn sl)))
   -> Empty Sp'
   -> Empty L'
-  -> discard_merge_sl slot (do_spill_rm slot sl)
-   = discard_merge_sl slot (do_spill_rm slot sl')
+  -> discard_merge_sl slot (do_spill_rm' slot n  sl)
+   = discard_merge_sl slot (do_spill_rm' slot n' sl')
 .
 Proof.
   intros top_sl' Empty_Sp Empty_L Empty_Sp' Empty_L'.
   rewrite top_sl'.
-  rewrite do_spill_rm_empty'';
+  rewrite do_spill_rm_empty;
     try rewrite getAnn_setTopAnn; eauto.
-  rewrite do_spill_rm_empty'';
+  rewrite do_spill_rm_empty;
     try rewrite getAnn_setTopAnn; eauto.
   unfold setTopAnn.
   do 2 rewrite discard_merge_sl_step.
   induction sl; simpl; destruct a; destruct p;
     simpl; reflexivity.
 Qed.
+*)
+Definition sub_spill
+           (sl' sl : ann (set var * set var * option (list (set var * set var))))
+  :=
+    sl' = setTopAnn sl (getAnn sl') (*Note that rm=rm' *)
+    /\ fst (fst (getAnn sl')) ⊆ fst (fst (getAnn sl))
+    /\ snd (fst (getAnn sl')) ⊆ snd (fst (getAnn sl))
+    /\ snd (getAnn sl') = snd (getAnn sl)
+.
 
 
+Lemma do_spill_rm_zero
+      (slot : var -> var)
+      (sl : ann (set var * set var * option (list (set var * set var))))
+  :
+    do_spill_rm' slot 0 sl
+    = match sl with
+       | ann0 (Sp, L, rm) => ann0 (Sp, L, rm)
+       | ann1 (Sp, L, rm) sl_s => ann1 (Sp, L, rm) (do_spill_rm slot sl_s)
+       | ann2 (Sp, L, rm) sl_s sl_t =>
+           ann2 (Sp, L, rm) (do_spill_rm slot sl_s) (do_spill_rm slot sl_t)
+       | annF (Sp, L, rm) sl_F sl_t =>
+           annF (Sp, L, rm) (do_spill_rm slot ⊝ sl_F) (do_spill_rm slot sl_t)
+       end
+.
+Proof.
+  unfold do_spill_rm'.
+  induction sl; fold do_spill_rm';
+    destruct a;
+    destruct p;
+    reflexivity.
+Qed.
+
+
+Lemma tl_list_incl
+      (X : Type) `{OrderedType X}
+      (L : list X)
+  :
+    of_list (tl L) ⊆ of_list L
+.
+Proof.
+  general induction L; simpl; eauto with cset.
+Qed.
+
+
+Lemma tl_set_incl
+      (X : Type) `{OrderedType X}
+      (s : set X)
+  :
+    of_list (tl (elements s)) ⊆ s
+.
+Proof.
+  rewrite tl_list_incl.
+  hnf. intros. eapply elements_iff. cset_tac.
+Qed.
+
+
+
+
+
+Lemma count_reduce_L
+      (sl : ann (set var * set var * option (list (set var * set var))))
+      (n m : nat)
+  :
+    count sl = S n
+    -> cardinal (snd (fst (getAnn sl))) = S m
+    -> count (setTopAnn sl (fst (fst (getAnn sl)),
+                           of_list (tl (elements (snd (fst (getAnn sl))))),
+                           snd (getAnn sl)))
+      = n
+.
+Proof.
+  intros count_sl card_L.
+  unfold count in *.
+  rewrite getAnn_setTopAnn.
+  simpl.
+  rewrite cardinal_set_tl with (n:=m).
+  - omega.
+  - rewrite of_list_elements. assumption.
+Qed.
+
+
+
+
+
+Lemma count_reduce_Sp
+      (sl : ann (set var * set var * option (list (set var * set var))))
+      (n m : nat)
+  :
+    count sl = S n
+    -> cardinal (fst (fst (getAnn sl))) = S m
+    -> count (setTopAnn sl (of_list (tl (elements (fst (fst (getAnn sl))))),
+                           snd (fst (getAnn sl)),
+                           snd (getAnn sl)))
+      = n
+.
+Proof.
+  intros count_sl card_Sp.
+  unfold count in *.
+  rewrite getAnn_setTopAnn.
+  simpl.
+  rewrite cardinal_set_tl with (n:=m).
+  - omega.
+  - rewrite of_list_elements. assumption.
+Qed.
 
 
 
 Lemma spill_live_sound_s
-(slot : var -> var) (*maybe needs restrictions*)
-(ZL : list params)
-(G : set var)
-(Λ : list (set var * set var))
-(Lv : list (set var))
-(s : stmt)
-(sl : ann (set var * set var * option (list (set var * set var))))
+      (slot : var -> var)
+      (n : nat)
+      (ZL : list params)
+      (G : set var)
+      (Λ : list (set var * set var))
+      (Lv : list (set var))
+      (s : stmt)
+      (sl sl': ann (set var * set var * option (list (set var * set var))))
   :
-  let sl' := setTopAnn sl (∅,∅,snd (getAnn sl)) in
-  (forall G', live_sound Imperative ZL Lv
-                (do_spill' slot s sl')
-                (spill_live (slot_merge slot Λ) ZL G'
-                            (do_spill' slot s sl')
-                            (discard_merge_sl slot (do_spill_rm slot sl')))
-  )
+    sub_spill sl' sl
+    -> n = count sl'
+    -> let sl0 := setTopAnn sl (∅,∅,snd (getAnn sl)) in
+   (forall G', live_sound Imperative ZL Lv
+              (do_spill slot s sl0)
+              (spill_live (slot_merge slot Λ) ZL G'
+                          (do_spill slot s sl0)
+                          (discard_merge_sl slot (do_spill_rm' slot 0 sl))))
 -> live_sound Imperative ZL Lv
-              (do_spill' slot s sl)
+              (do_spill slot s sl')
               (spill_live (slot_merge slot Λ) ZL G
-                          (do_spill' slot s sl)
-                          (discard_merge_sl slot (do_spill_rm slot sl))).
+                          (do_spill slot s sl')
+                          (discard_merge_sl slot (do_spill_rm' slot n sl))).
 Proof.
 
-set (Sp := fst (fst (getAnn sl))).
-set (L  := snd (fst (getAnn sl))).
-set (rm := snd (getAnn sl)).
-intros sl' strong_sls.
+set (Sp' := fst (fst (getAnn sl'))).
+set (L'  := snd (fst (getAnn sl'))).
+set (rm' := snd (getAnn sl')).
+intros sub_sl n_count sl0 strong_sls.
 
-
-remember (cardinal Sp) as n_Sp.
-symmetry in Heqn_Sp.
-revert dependent sl.
+remember (cardinal Sp') as n_Sp'.
+symmetry in Heqn_Sp'.
+rename Heqn_Sp' into card_Sp'.
+revert dependent sl'.
 revert G.
-induction n_Sp;
-  intros G sl Sp L rm sl' strong_sls card_Sp.
+revert n.
+induction n_Sp';
+  intros n G sl' Sp' L' rm' sub_sl n_count card_Sp'.
 
-- remember (cardinal L) as n_L.
-  symmetry in Heqn_L.
-  revert dependent sl.
+- remember (cardinal L') as n_L'.
+  symmetry in Heqn_L'.
+  rename Heqn_L' into card_L'.
+  revert dependent sl'.
   revert G.
-  induction n_L;
-    intros G sl Sp L rm sl' strong_sls card_Sp card_L.
+  revert n.
+  induction n_L';
+    intros n G sl' Sp' L' rm' sub_sl n_count card_Sp' card_L'.
 
   {
+    assert (count sl' = 0) as count_sl'.
+    { unfold count. subst Sp'. subst L'.
+      rewrite card_Sp'. rewrite card_L'. omega. }
     rewrite do_spill_empty_invariant
-    with (Sp':=∅) (L':=∅) (rm:=rm) (sl':=sl');
-      subst Sp; subst L; simpl; eauto; try apply empty_1;
+    with (Sp':=∅) (L':=∅) (rm:=rm') (sl':=sl0);
+      simpl; eauto; try apply empty_1;
       try apply cardinal_Empty; eauto.
-    + rewrite dms_dsr_empty_invariant
-      with (Sp':=∅) (L':=∅) (sl':=sl');
-        eauto; try apply empty_1;
-        apply cardinal_Empty; assumption.
+
+    + rewrite n_count.
+      rewrite count_sl'.
+      rewrite do_spill_rm_zero.
+      destruct sl; destruct a; destruct p; apply strong_sls.
+    + subst sl0.
+      unfold sub_spill in sub_sl.
+      destruct  sub_sl as [top_sl' [sub_Sp [sub_L eq_rm]]].
+      rewrite <- eq_rm.
+      rewrite top_sl'.
+      rewrite setTopAnn_setTopAnn.
+      rewrite getAnn_setTopAnn.
+      subst rm'.
+      reflexivity.
   }
 
-  rewrite do_spill_rm_s with (n:=n_L).
-  Focus 2. subst Sp. rewrite card_Sp.
-           subst L. rewrite card_L.
-           omega.
 
   rewrite do_spill_L.
-  Focus 2. subst Sp. rewrite cardinal_Empty. assumption.
-  Focus 2. subst L. clear - card_L. intro N.
-           apply cardinal_Empty in N. omega.
+  Focus 2. rewrite cardinal_Empty. subst Sp'. assumption.
+  Focus 2. clear - card_L'. intro N.
+           apply cardinal_Empty in N. subst L'. omega.
 
-  econstructor; fold spill_live.
-  * assert (forall sl, add_nones n_L
-              match sl with
-              | ann0 (Sp, L, rm) => ann0 (Sp, L, rm)
-              | ann1 (Sp, L, rm) sl_s => ann1 (Sp, L, rm) (do_spill_rm slot sl_s)
-              | ann2 (Sp, L, rm) sl_s sl_t =>
-                  ann2 (Sp, L, rm) (do_spill_rm slot sl_s) (do_spill_rm slot sl_t)
-              | annF (Sp, L, rm) sl_F sl_t =>
-                  annF (Sp, L, rm) (do_spill_rm slot ⊝ sl_F) (do_spill_rm slot sl_t)
-              end
-              = do_spill_rm slot
-                   (setTopAnn sl (fst (fst (getAnn sl)),
-                                  of_list (tl (elements (snd (fst (getAnn sl))))),
-                                  snd (getAnn sl)
-                                 )
-                   )
-             ) as eq_dsr.
-    {
-      admit. (* solvable, maybe complicated *)
-    }
-    rewrite eq_dsr. clear eq_dsr.
-    apply IHn_L.
-    -- rewrite setTopAnn_setTopAnn.
-       rewrite getAnn_setTopAnn.
-       subst sl'. subst rm.
+  rewrite n_count.
+  unfold count.
+  subst Sp'.
+  subst L'.
+  rewrite card_L'.
+  rewrite card_Sp'.
+  simpl.
+
+  rewrite do_spill_rm_s.
+
+  rewrite discard_merge_sl_step.
+
+  constructor; fold spill_live.
+
+  * apply IHn_L'.
+    -- unfold sub_spill.
+       unfold sub_spill in sub_sl.
+       destruct sub_sl as [top_sl' [sub_Sp [sub_L eq_rm]]].
+       repeat split; rewrite getAnn_setTopAnn; simpl; eauto.
+       ++ rewrite top_sl'. rewrite setTopAnn_setTopAnn.
+          rewrite getAnn_setTopAnn. reflexivity.
+       ++ rewrite tl_set_incl. assumption.
+
+    -- rewrite count_reduce_L with (n:=n_L') (m:=n_L'); eauto.
+       unfold count. rewrite card_Sp'. rewrite card_L'. eauto.
+    -- rewrite getAnn_setTopAnn.
        simpl.
-       apply strong_sls.
+       assumption.
     -- rewrite getAnn_setTopAnn.
-       simpl. subst Sp. assumption.
-    -- rewrite getAnn_setTopAnn.
-       simpl. admit. (* okay, needs lemma:          cardinal L = S n_L
-                     -> cardinal (of_list (tl (elements (L)))) =   n_L *)
+       simpl. erewrite cardinal_set_tl. eauto.
+       rewrite of_list_elements. rewrite card_L'. eauto.
     * apply live_exp_sound_incl
         with (lv':=Exp.freeVars (Operation (Var (slot
-                         (hd 0 (elements (snd (fst (getAnn sl))))))))).
+                         (hd 0 (elements (snd (fst (getAnn sl'))))))))).
       -- apply live_freeVars.
       -- clear. cset_tac.
     * clear. cset_tac.
     * apply spill_live_G.
 
-- rewrite do_spill_rm_s with (n:=n_Sp + cardinal L).
-  Focus 2. subst Sp. rewrite card_Sp.
-           subst L. omega.
-
-  rewrite do_spill_Sp. (*Lemma not yet proven*)
-  Focus 2. subst Sp. clear - card_Sp. intro N.
+- rewrite do_spill_Sp.
+  Focus 2. subst Sp'. clear - card_Sp'. intro N.
            apply cardinal_Empty in N. omega.
 
+  rewrite n_count.
+  unfold count.
+  subst Sp'.
+  rewrite card_Sp'.
+  simpl.
+
+
+  rewrite do_spill_rm_s with (n:=n_Sp' + cardinal L').
+
   econstructor; fold spill_live.
-  * assert (forall sl, add_nones (n_Sp + cardinal L)
-              match sl with
-              | ann0 (Sp, L, rm) => ann0 (Sp, L, rm)
-              | ann1 (Sp, L, rm) sl_s => ann1 (Sp, L, rm) (do_spill_rm slot sl_s)
-              | ann2 (Sp, L, rm) sl_s sl_t =>
-                  ann2 (Sp, L, rm) (do_spill_rm slot sl_s) (do_spill_rm slot sl_t)
-              | annF (Sp, L, rm) sl_F sl_t =>
-                  annF (Sp, L, rm) (do_spill_rm slot ⊝ sl_F) (do_spill_rm slot sl_t)
-              end
-              = do_spill_rm slot
-                   (setTopAnn sl (of_list (tl (elements (fst (fst (getAnn sl))))),
-                                  snd (fst (getAnn sl)),
-                                  snd (getAnn sl)
-                                 )
-                   )
-             ) as eq_dsr.
-    {
-      admit. (* solvable, maybe complicated *)
-    }
-    rewrite eq_dsr. clear eq_dsr.
-    apply IHn_Sp.
-    -- rewrite setTopAnn_setTopAnn.
-       rewrite getAnn_setTopAnn.
-       subst sl'. subst rm.
-       simpl.
-       apply strong_sls.
+  * apply IHn_Sp'.
+    -- unfold sub_spill.
+       unfold sub_spill in sub_sl.
+       destruct sub_sl as [top_sl' [sub_Sp [sub_L eq_rm]]].
+       repeat split; rewrite getAnn_setTopAnn; simpl; eauto.
+       ++ rewrite top_sl'. rewrite setTopAnn_setTopAnn.
+          rewrite getAnn_setTopAnn. reflexivity.
+       ++ rewrite tl_set_incl. assumption.
+    -- rewrite count_reduce_Sp with (n:=n_Sp' + cardinal L') (m:=n_Sp'); eauto.
+       unfold count. rewrite card_Sp'. subst L'. omega.
     -- rewrite getAnn_setTopAnn.
-       simpl. admit. (* okay, needs lemma:   cardinal L = S n_L
-                     -> cardinal (of_list (tl (elements (L)))) =   n_L *)
-    * apply live_exp_sound_incl
-        with (lv':=Exp.freeVars (Operation (Var (
-                         (hd 0 (elements (snd (fst (getAnn sl))))))))).
-      -- apply live_freeVars.
+       simpl.
+       erewrite cardinal_set_tl; eauto.
+       rewrite of_list_elements.
+       rewrite card_Sp'.
+       omega.
+     * apply live_exp_sound_incl
+        with (lv':= singleton (hd 0 (elements (fst (fst (getAnn sl')))))).
+      -- econstructor. econstructor. eauto with cset.
       -- clear. cset_tac.
     * clear. cset_tac.
     * apply spill_live_G.
-Admitted.
+Qed.
 
+
+Lemma sub_spill_refl sl
+  :
+    sub_spill sl sl
+.
+Proof.
+  unfold sub_spill.
+  repeat split.
+    simpl; eauto.
+  - unfold setTopAnn.
+    destruct sl; destruct a; destruct p;
+      simpl; reflexivity.
+  - reflexivity.
+  - reflexivity.
+Qed.
 
 Lemma spill_live_sound
 (k : nat)
-(slot : var -> var) (*maybe needs restrictions*)
+(slot : var -> var)
+(n : nat)
 (ZL : list params)
 (G : set var)
 (Λ : list (set var * set var))
@@ -901,35 +633,22 @@ Lemma spill_live_sound
 -> spill_sound k ZL Λ (R,M) s sl
 -> live_sound Imperative ZL Lv s alv
 -> live_sound Imperative ZL Lv
-              (do_spill' slot s sl)
+              (do_spill slot s sl)
               (spill_live (slot_merge slot Λ) ZL G
-                          (do_spill' slot s sl)
+                          (do_spill slot s sl)
                           (discard_merge_sl slot (do_spill_rm slot sl))).
 
 Proof.
 intros aeFree spillSound lvSound.
-(*induction (elements (fst (fst (getAnn sl)))).
-general induction spillSound; inversion_clear lvSound; inversion_clear aeFree;
-simpl.
- *)
-(*
-set (Sp := fst (fst (getAnn sl))).
-set (L  := snd (fst (getAnn sl))).
-set (rm := snd (getAnn sl)).
-assert (getAnn sl = (Sp,L,rm)) as gA_sl.
-{ induction sl; simpl in *; destruct a as [[Sp' L'] rm'];
-    subst Sp; subst L; subst rm; simpl; reflexivity.
-}
- *)
+
 general induction lvSound;
   inversion_clear aeFree;
   inversion_clear spillSound;
-  apply spill_live_sound_s; intros G'.
+  apply spill_live_sound_s;
+  try apply sub_spill_refl; eauto.
 - rewrite do_spill_empty.
-  rewrite do_spill_rm_empty''.
+  rewrite do_spill_rm_zero.
   rewrite discard_merge_sl_step; simpl.
-  Focus 2. simpl. apply empty_1.
-  Focus 2. simpl. apply empty_1.
   Focus 2. simpl. apply empty_1.
   Focus 2. simpl. apply empty_1.
 
@@ -941,10 +660,8 @@ general induction lvSound;
   +  clear. cset_tac.
   + apply spill_live_G.
 - rewrite do_spill_empty.
-  rewrite do_spill_rm_empty''.
+  rewrite do_spill_rm_zero.
   rewrite discard_merge_sl_step; simpl.
-  Focus 2. simpl. apply empty_1.
-  Focus 2. simpl. apply empty_1.
   Focus 2. simpl. apply empty_1.
   Focus 2. simpl. apply empty_1.
 
@@ -958,10 +675,8 @@ general induction lvSound;
   + clear. cset_tac.
 - admit.
 - rewrite do_spill_empty.
-  rewrite do_spill_rm_empty''.
+  rewrite do_spill_rm_zero.
   rewrite discard_merge_sl_step; simpl.
-  Focus 2. simpl. apply empty_1.
-  Focus 2. simpl. apply empty_1.
   Focus 2. simpl. apply empty_1.
   Focus 2. simpl. apply empty_1.
 
@@ -972,407 +687,3 @@ general induction lvSound;
 - admit.
 
 Admitted.
-
-
-enough (forall Sp' sl', Sp' ⊆ Sp
-          -> sl'= setTopAnn sl (Sp',L,rm)
-          -> live_sound Imperative ZL Lv (do_spill' slot s sl')
-                    (spill_live (slot_merge slot Λ) ZL G (do_spill' slot s sl')
-                                (discard_merge_sl slot (do_spill_rm slot sl')))
-       ) as strong_Sp_sls.
-{
-  apply strong_Sp_sls with (Sp':=Sp).
-  - eauto with cset.
-  - symmetry. apply setTopAnn_eta. eauto.
-}
-
-intros Sp' sl' sub_Sp top_sl'.
-assert (Sp' = fst (fst (getAnn sl'))) as HeqSp'.
-{ rewrite top_sl'. rewrite getAnn_setTopAnn. simpl. eauto. }
-assert (getAnn sl' = (Sp',L,rm)) as gA_sl'.
-{
-  rewrite top_sl'. rewrite getAnn_setTopAnn. reflexivity.
-}
-
-remember (cardinal Sp') as n_Sp'.
-symmetry in Heqn_Sp'.
-revert dependent sl'. revert dependent Sp'. revert G.
-induction n_Sp'; intros G Sp' sub_Sp card_Sp' sl' top_sl' HeqSp' gA_sl'.
-- enough (forall L' sl'', L' ⊆ L
-           -> sl'' = setTopAnn sl' (Sp',L',rm)
-           -> live_sound Imperative ZL Lv (do_spill' slot s sl'')
-                    (spill_live (slot_merge slot Λ) ZL G (do_spill' slot s sl'')
-                                (discard_merge_sl slot (do_spill_rm slot sl'')))
-         ) as strong_L_sls.
-  {
-    apply strong_L_sls with (L':=L).
-    - eauto with cset.
-    - symmetry. apply setTopAnn_eta. eauto.
-  }
-  intros L' sl'' sub_L top_sl''.
-  assert (L' = snd (fst (getAnn sl''))) as HeqL'.
-  { rewrite top_sl''. rewrite getAnn_setTopAnn. simpl. eauto. }
-  assert (Sp'= fst (fst (getAnn sl''))) as HeqSp''.
-  { rewrite top_sl''. rewrite getAnn_setTopAnn. simpl. eauto. }
-  assert (getAnn sl'' = (Sp',L',rm)) as gA_sl''.
-  {
-    rewrite top_sl''. rewrite getAnn_setTopAnn. reflexivity.
-  }
-
-  remember (cardinal L') as n_L'.
-  symmetry in Heqn_L'.
-  revert dependent sl''.
-  revert dependent L'.
-  revert G.
-  induction n_L'; intros G L' sub_L card_L' sl'' top_sl'' HeqL' HeqSp'' gA_sl''.
-
-  + assert (sl'' = setTopAnn sl (Sp',L',rm)) as top_sl.
-    { rewrite top_sl''. rewrite top_sl'. rewrite setTopAnn_setTopAnn. eauto. }
-
-    revert dependent sl''.
-    revert spillSound.
-    revert G R M.
-    induction lvSound; intros G R M spillSound sl'';
-      inversion_clear spillSound; inversion_clear aeFree;
-        intros top_sl'' HeqL'' HeqSp'' gA_sl'' top_sl.
-    * (*cbn zeta. intros _ sub_Sp Heq_sl' gA_sl' sub_L top_sl'' gA_sl'' Heq_sl''.*)
-      simpl in sub_Sp, gA_sl', sub_L, top_sl'', gA_sl''.
-      rewrite do_spill_empty.
-      rewrite do_spill_rm_empty''.
-      rewrite discard_merge_sl_step; simpl.
-      rewrite top_sl.
-      simpl.
-      Focus 2. apply cardinal_Empty. rewrite <- HeqSp''. assumption.
-      Focus 2. apply cardinal_Empty. rewrite <- HeqL''.  assumption.
-      Focus 2. apply cardinal_Empty. rewrite <- HeqSp''. assumption.
-      Focus 2. apply cardinal_Empty. rewrite <- HeqL''.  assumption.
-      destruct rm ; econstructor.
-      -- apply IHlvSound with (R:={x; R\K∪L0}) (M:=Sp0∪M); eauto.
-         ++ econstructor.
-      -- admit.
-      -- admit.
-      -- admit.
-    * admit.
-    * admit.
-    * admit.
-    * admit.
-    (*
-    revert dependent R.
-    revert dependent M.
-    induction lvSound.
-    * simpl.
-    assert (cardinal Sp = 0 /\ cardinal L = 0) as [card_Sp card_L].
-    { clear - Heqn. split; omega. }
-    assert (Empty Sp /\ Empty L) as [Empty_Sp Empty_L].
-    { clear - card_Sp card_L. split; apply cardinal_Empty; eauto. }
-    assert (elements Sp = nil /\ elements L = nil) as [nil_Sp nil_L].
-    { split; apply elements_Empty; eauto. }
-
-    rewrite nil_Sp. rewrite nil_L.
-    rewrite write_spills_empty. rewrite write_loads_empty.
-
-
-    rewrite <- Heqn. unfold add_nones.
-    rewrite discard_merge_sl_1.
-    simpl. econstructor.
-    * eapply IHlvSound; eauto.
-    * apply live_exp_sound_incl with (lv':=Exp.freeVars e).
-      -- apply Exp.live_freeVars.
-      -- clear. cset_tac.
-    * clear. cset_tac.
-    * apply spill_live_G. *)
-
-  + rewrite do_spill_rm_s with (n:=n_L').
-    Focus 2. rewrite <- HeqL'. rewrite <- HeqSp''.
-             rewrite card_Sp'. rewrite card_L'. omega.
-
-    rewrite do_spill_L. (* Lemma not yet proven *)
-    Focus 2. rewrite <- HeqSp''. apply cardinal_Empty. eauto.
-    Focus 2. rewrite <- HeqL'. clear - card_L'.
-             intro N. apply cardinal_Empty in N. omega.
-
-    econstructor; fold spill_live.
-    * assert (forall sl, add_nones n_L'
-              match sl with
-              | ann0 (Sp, L, rm) => ann0 (Sp, L, rm)
-              | ann1 (Sp, L, rm) sl_s => ann1 (Sp, L, rm) (do_spill_rm slot sl_s)
-              | ann2 (Sp, L, rm) sl_s sl_t =>
-                  ann2 (Sp, L, rm) (do_spill_rm slot sl_s) (do_spill_rm slot sl_t)
-              | annF (Sp, L, rm) sl_F sl_t =>
-                  annF (Sp, L, rm) (do_spill_rm slot ⊝ sl_F) (do_spill_rm slot sl_t)
-              end
-              = do_spill_rm slot
-                   (setTopAnn sl (fst (fst (getAnn sl)),
-                                  of_list (tl (elements (snd (fst (getAnn sl))))),
-                                  snd (getAnn sl)
-                                 )
-                   )
-             ) as eq_dsr.
-      {
-        admit. (* solvable, maybe complicated *)
-      }
-      rewrite eq_dsr. clear eq_dsr.
-      apply IHn_L' with (L':=of_list (tl (elements (snd (fst (getAnn sl''))))));
-        simpl; eauto.
-
-      -- rewrite <- HeqL'. admit. (* easy *) (* needs lemma of_list_monotone *)
-      -- rewrite <- HeqL'. admit. (* okay *) (* needs lemma of_list_tl_subset *)
-      -- rewrite <- HeqSp''. rewrite <- HeqL'.
-         rewrite gA_sl''. simpl. eauto.
-         rewrite top_sl''. rewrite setTopAnn_setTopAnn. eauto.
-      -- rewrite getAnn_setTopAnn. simpl. eauto.
-      -- rewrite getAnn_setTopAnn. simpl. eauto.
-      -- rewrite getAnn_setTopAnn. rewrite <- HeqSp''.
-         rewrite <- HeqL'. rewrite gA_sl''. simpl. eauto.
-
-    * apply live_exp_sound_incl
-        with (lv':=Exp.freeVars (Operation (Var (slot
-                         (hd 0 (elements (snd (fst (getAnn sl''))))))))).
-      -- apply live_freeVars.
-      -- clear. cset_tac.
-    * rewrite <- HeqSp''. rewrite <- HeqL'. clear. cset_tac.
-      (* this is not performant *)
-    * apply spill_live_G.
-
-- rewrite do_spill_rm_s with (n:=n_Sp').
-  admit. admit. (* analogous *)
-
-Admitted.
-
-
-
-Print Syntax error: '.' expected after [vernac:command] (in [vernac_aux]).
-
-
-
-
-
-
-
-
-
-
-
-
-
-
-
-
-general induction lvSound;  inversion_clear spillSound;
-
-inversion_clear aeFree as [x' e' s' eaFree_s
-                          |e'
-                          |e' s' t' aeFree_s eaFree_t
-                          |f' Y' aeFree_var
-                          |F' t' aeFree_F aeFree_t];
- clear sl; try rename sl0 into sl.
-
-- remember (elements Sp) as xs.  remember (elements L) as ys.
-  remember (cardinal Sp + cardinal L) as n.
-  revert dependent Sp.
-  revert dependent L.
-  induction n; intros.
-  + simpl.
-    assert (cardinal Sp = 0 /\ cardinal L = 0) as [card_Sp card_L].
-    { clear - Heqn. split; omega. }
-    assert (Empty Sp /\ Empty L) as [Empty_Sp Empty_L].
-    { clear - card_Sp card_L. split; apply cardinal_Empty; eauto. }
-    assert (elements Sp = nil /\ elements L = nil) as [nil_Sp nil_L].
-    { split; apply elements_Empty; eauto. }
-
-    rewrite nil_Sp. rewrite nil_L.
-    rewrite write_spills_empty. rewrite write_loads_empty.
-
-
-    rewrite <- Heqn. unfold add_nones.
-    rewrite discard_merge_sl_1.
-    simpl. econstructor.
-    * eapply IHlvSound; eauto.
-    * apply live_exp_sound_incl with (lv':=Exp.freeVars e).
-      -- apply Exp.live_freeVars.
-      -- clear. cset_tac.
-    * clear. cset_tac.
-    * apply spill_live_G.
-
-  + assert (cardinal Sp > 0 \/ cardinal L > 0) as SpL_non_zero.
-    {
-      clear - Heqn. decide (cardinal Sp = 0).
-      - right. rewrite e in Heqn. simpl in Heqn. omega.
-      - left. omega.
-    }
-    simpl.
-    rewrite <- Heqxs. rewrite <- Heqys.
-    change (add_nones (cardinal Sp + cardinal L) (ann1 (Sp, L, ⎣⎦) (do_spill_rm slot sl)))
-           with (do_spill_rm slot (ann1 (Sp,L,None) sl)).
-    rewrite do_spill_rm_s with (n:=cardinal Sp + cardinal L - 1).
-
-    Focus 2.
-      simpl.
-      assert (cardinal Sp + cardinal L > 0) as SpL_gt0.
-      { clear - Heqn. omega. }
-      omega.
-
-    rewrite discard_merge_sl_1.
-    simpl.
-    destruct xs.
-    * simpl. destruct ys.
-      -- admit. (* see above *)
-      -- simpl. econstructor.
-         ++ replace (write_loads slot ys (stmtLet x e (do_spill slot s sl)))
-               with (do_spill slot (stmtLet x e s) (ann1 (∅,of_list ys,None) sl)).
-            (*change (add_nones (cardinal Sp + cardinal L - 1)
-                              (ann1 (Sp,L,None) (do_spill_rm slot sl)))
-                   with (do_spill_rm slot (ann1 (Sp,L,None) sl)).
-            apply IHn. *) admit. admit.
-         ++
-
-  (* *)
-
-  induction xs,ys.
-  + simpl.
-    rewrite <- Heqxs. rewrite write_spills_empty.
-    rewrite <- Heqys. rewrite write_loads_empty.
-
-    change (live_sound Imperative ZL Lv (stmtLet x e (do_spill slot s sl))
-             (spill_live (slot_merge slot Λ) ZL G (stmtLet x e (do_spill slot s sl))
-               (discard_merge_sl slot (do_spill_rm slot (ann1 (Sp,L,None) sl))))).
-
-    assert (  discard_merge_sl slot (do_spill_rm slot (ann1 (Sp,L,None) sl))
-            = discard_merge_sl slot((ann1 (Sp,L,None) (do_spill_rm slot sl))))
-                  as dms.
-    {
-      rewrite do_spill_rm_empty''; simpl; eauto.
-      - apply elements_Empty. eauto.
-      - apply elements_Empty. eauto.
-    }
-
-    rewrite dms.
-    rewrite discard_merge_sl_1.
-    simpl. econstructor.
-
-    * eapply IHlvSound; eauto.
-    * apply live_exp_sound_incl with (lv':=Exp.freeVars e).
-      -- apply Exp.live_freeVars.
-      -- cset_tac.
-    * cset_tac.
-    * apply spill_live_G.
-
-  + simpl.
-    rewrite <- Heqxs. simpl.
-    rewrite <- Heqys. unfold write_loads. fold write_loads.
-    change (live_sound Imperative ZL Lv
-     (stmtLet v (Operation (Var (slot v)))
-        (write_loads slot ys (stmtLet x e (do_spill slot s sl))))
-     (spill_live (slot_merge slot Λ) ZL G
-        (stmtLet v (Operation (Var (slot v)))
-           (write_loads slot ys (stmtLet x e (do_spill slot s sl))))
-        (discard_merge_sl slot
-           (do_spill_rm slot (ann1 (Sp,L,None) sl))))).
-
-    rewrite do_spill_rm_s with (n:= cardinal Sp + cardinal L - 1).
-    Focus 2. simpl. admit.
-    rewrite discard_merge_sl_1.
-
-    simpl. econstructor.
-    * admit. (* difficult *)
-    * apply live_exp_sound_incl with (lv':=singleton (slot v)).
-      -- econstructor. econstructor. cset_tac.
-      -- cset_tac.
-    * cset_tac.
-    * apply spill_live_G.
-
-
-
-         rewrite <- write_spills_empty
-        with (slot:=slot) (s:=write_loads slot ys (stmtLet x e (do_spill slot s sl))).
-
-      replace (write_spills slot nil (write_loads slot ys (stmtLet x e (do_spill slot s sl))))
-      with (do_spill slot (stmtLet x e s) (ann1 (∅,of_list ys,None) sl)).
-
-      eapply IHlvSound; eauto.
-    assert ( do_spill_rm slot (ann1 (Sp,L,None) sl)
-           = ann1 (∅,∅,None)
-                  (do_spill_rm slot (ann1 (∅,of_list ys,None) sl))) as dms_cons.
-    {
-      rewrite do_spill_rm_s with (n:=cardinal Sp + cardinal L).
-      Focus 2. simpl.
-      -
-
-
-(*+TODO+*)
-
-    rewrite annEq.
-    replace (((fix f (n : nat) (b : ann (⦃var⦄ * ⦃var⦄ * ؟ 〔⦃var⦄ * ⦃var⦄〕)) {struct n} :
-               ann (⦃var⦄ * ⦃var⦄ * ؟ 〔⦃var⦄ * ⦃var⦄〕) :=
-               match n with
-               | 0 => b
-               | S n0 => ann1 (∅, ∅, ⎣⎦) (f n0 b)
-               end) (cardinal Sp + cardinal L) (ann1 (Sp, L, ⎣⎦) (do_spill_rm slot sl)))) with (ann1 (∅,∅,None) (do_spill_rm slot sl)).
-    Focus 2. rewrite emptySp. rewrite emptyL.
-    apply do_spill_rm_empty.
-    simpl.
-    rewrite emptySp. rewrite emptyL.
-    econstructor.
-    * eapply IHspillSound; eauto.
-    * apply live_exp_sound_incl with (lv':=Exp.freeVars e).
-      -- apply Exp.live_freeVars.
-      -- cset_tac.
-    * eauto.
-    * admit.
-  + rewrite write_spills_empty.
-    rewrite write_spills_empty in IHl.
-    simpl. econstructor.
-    * admit.
-    * econstructor. econstructor. cset_tac.
-    * eauto.
-    * revert a. admit. (*this is unprovable*)
-  + rewrite write_loads_empty.
-    rewrite write_loads_empty in IHl.
-    simpl. econstructor.
-    * admit.
-    * econstructor. econstructor. cset_tac.
-    * eauto.
-    * admit. (*this is unprovable*)
-  + admit.
-- induction (elements Sp); induction (elements L).
-  + rewrite write_loads_empty. rewrite write_spills_empty.
-    simpl. econstructor. apply Op.live_freeVars.
-  + rewrite write_spills_empty.
-    rewrite write_spills_empty in IHl.
-    simpl. eapply LOpr.
-
-- apply live_exp_sound_incl with (lv':=Exp.freeVars e).
-  + apply Exp.live_freeVars.
-  + cset_tac.
-- admit.
-- admit.
-- econstructor. econstructor. cset_tac.
-- simpl. induction (elements Sp), (elements L); simpl.
-  + econstructor; eauto.
-    * apply live_exp_sound_incl with (lv':=Exp.freeVars e).
-      -- apply Exp.live_freeVars.
-      -- cset_tac.
-    * admit. (*Why do we need this condition?*)
-  + admit.
-  + admit.
-  + admit.
-- apply do_spill_empty_if in IHlvSound1.
-  apply do_spill_empty_if.
-  +
-enough (forall sl1 sl2, live_sound Imperative ZL Lv (do_spill slot s1
-   (ann2 (∅,∅,None) sl1 sl2))
-   (spill_live slot Λ ZL (do_spill slot s1 (ann2 (∅,∅,None) sl1 sl2))
-                                           (ann2 (∅,∅,None) sl1 sl2))
-  -> live_sound Imperative ZL Lv (stmtIf e ).
-   * apply H8.
-eapply IHlvSound1. ; admit.
-- econstructor; admit.
-- econstructor. apply Op.live_freeVars.
-- econstructor; admit.
-
-Op.live_freeVars
-
-Theorem spill_sound_correct L E E' : spill_sound k Lsl (R,M) s alv asl
--> (forall x : var, In x R -> E x = E' x)
--> (forall x : var, In x S -> E x = E' (slot x))
--> sim'r Bisim (L,E,s) (L,E', doSpill slot s asl).
