theories/Spilling/DoSpill.v
@@ -1,0 +1,195 @@
+Require Import List Map Env AllInRel Exp AppExpFree.
+Require Import IL Annotation InRel AutoIndTac Liveness LabelsDefined.
+Require Import SimI Spilling.
+
+Fixpoint do_spill
+         (slot : var -> var)
+         (s : stmt)
+         (sl0 : ann (set var * set var * option(list(set var * set var))))
+         {struct s}
+  : stmt :=
+
+
+
+  let Sp0 := fst (fst (getAnn sl0)) in
+  let L0  := snd (fst (getAnn sl0)) in
+  let rm  := snd (getAnn sl0) in
+
+(fix f sl n {struct n} :=
+  let Sp := fst (fst (getAnn sl)) in
+  let L  := snd (fst (getAnn sl)) in
+  match n with
+    | 0 =>
+     match s,sl with
+     | stmtLet x e s, ann1 _ sl_s
+       => stmtLet x e (do_spill slot s sl_s)
+     | stmtIf e s t, ann2 _ sl_s sl_t
+       => stmtIf e (do_spill slot s sl_s) (do_spill slot t sl_t)
+     | stmtFun F t, annF _ sl_F sl_t
+       => stmtFun
+            ((fun Zs sl_s => (fst Zs (* todo: really? I think it's fine *)
+                                    , do_spill slot (snd Zs) sl_s)) ⊜ F sl_F)
+                           (do_spill slot t sl_t)
+
+     | _,_
+       => s
+     end
+    | S n =>
+
+  if
+    [cardinal Sp = 0]
+  then
+    if
+      [cardinal L = 0]
+    then
+     match s,sl with
+     | stmtLet x e s, ann1 _ sl_s
+       => stmtLet x e (do_spill slot s sl_s)
+     | stmtIf e s t, ann2 _ sl_s sl_t
+       => stmtIf e (do_spill slot s sl_s) (do_spill slot t sl_t)
+     | stmtFun F t, annF _ sl_F sl_t
+       => stmtFun
+            ((fun Zs sl_s => (fst Zs (* todo: really? I think it's fine *)
+                                    , do_spill slot (snd Zs) sl_s)) ⊜ F sl_F)
+                           (do_spill slot t sl_t)
+
+     | _,_
+       => s
+     end
+
+    else
+      let x := hd 0 (elements L) in
+      let L':= of_list (tl (elements L)) in
+      stmtLet x (Operation (Var (slot x))) (f (setTopAnn sl (Sp,L',rm)) n)
+
+  else
+    let x  := hd 0 (elements Sp) in
+    let Sp':= of_list (tl (elements Sp)) in
+    stmtLet (slot x) (Operation (Var x)) (f (setTopAnn sl (Sp',L,rm)) n)
+  end
+) sl0 (cardinal Sp0 + cardinal L0)
+.
+
+
+
+Lemma do_spill_empty
+      (slot : var -> var)
+      (s : stmt)
+      (sl : ann (set var * set var * option (list (set var * set var))))
+  :
+    Empty (fst (fst (getAnn sl)))
+    -> Empty (snd (fst (getAnn sl)))
+    -> do_spill slot s sl
+      =
+
+      match s,sl with
+     | stmtLet x e s, ann1 _ sl_s
+       => stmtLet x e (do_spill slot s sl_s)
+     | stmtIf e s t, ann2 _ sl_s sl_t
+       => stmtIf e (do_spill slot s sl_s) (do_spill slot t sl_t)
+     | stmtFun F t, annF _ sl_F sl_t
+       => stmtFun
+            ((fun Zs sl_s => (fst Zs, do_spill slot (snd Zs) sl_s)) ⊜ F sl_F)
+            (do_spill slot t sl_t)
+
+     | _,_
+       => s
+      end.
+Proof.
+  intros Empty_Sp Empty_L.
+  remember (fst (fst (getAnn sl))) as Sp.
+  remember (snd (fst (getAnn sl))) as L.
+  assert (cardinal Sp = 0) as zero_Sp.
+  { apply cardinal_Empty. eauto. }
+  assert (cardinal L = 0) as zero_L.
+  { apply cardinal_Empty. eauto. }
+  induction sl, s; simpl in *; rewrite <- HeqSp; rewrite <- HeqL;
+    simpl; rewrite zero_Sp; rewrite zero_L; simpl; eauto.
+Qed.
+
+
+
+
+
+Lemma do_spill_Sp
+      (slot : var -> var)
+      (s : stmt)
+      (sl : ann (set var * set var * option (list (set var * set var))))
+  :
+    let Sp := fst (fst (getAnn sl)) in
+    let L  := snd (fst (getAnn sl)) in
+    let x  := hd 0 (elements Sp) in
+    let Sp':= of_list (tl (elements Sp)) in
+    ~ Empty Sp
+    -> do_spill slot s sl
+      = stmtLet (slot x)
+                (Operation (Var x))
+                (do_spill slot s (setTopAnn sl (Sp',L,snd (getAnn sl))))
+.
+Proof.
+  intros Sp L x Sp' NEmpty_Sp.
+  assert (~ cardinal Sp = 0) as Sp_nonzero.
+  { intro N. apply NEmpty_Sp. rewrite cardinal_Empty. eauto. }
+  assert (exists n, cardinal Sp = S n) as [n card_Sp].
+  { exists (cardinal Sp - 1). omega. }
+  subst Sp.
+  subst L.
+  assert (forall (t : set var), (S n) + cardinal t = S (n + cardinal t)) as nL_card_S.
+  { intros t. omega. }
+  induction s;
+    simpl;
+    rewrite card_Sp;
+    rewrite nL_card_S;
+    rewrite getAnn_setTopAnn;
+    rewrite card_Sp;
+    simpl;
+    subst x;
+    subst Sp';
+    rewrite cardinal_tl with (n:=n);
+    eauto;
+    reflexivity.
+Qed.
+
+Lemma do_spill_L
+      (slot : var -> var)
+      (s : stmt)
+      (sl : ann (set var * set var * option (list (set var * set var))))
+  :
+    let Sp := fst (fst (getAnn sl)) in
+    let L  := snd (fst (getAnn sl)) in
+    let x  := hd 0 (elements L) in
+    let L' := of_list (tl (elements L)) in
+    Empty Sp
+    -> ~ Empty L
+    -> do_spill slot s sl
+      = stmtLet x
+                (Operation (Var (slot x)))
+                (do_spill slot s (setTopAnn sl (Sp,L',snd (getAnn sl))))
+.
+Proof.
+  intros Sp L x L' Empty_Sp NEmpty_L.
+  assert (~ cardinal L = 0) as L_nonzero.
+  { intro N. apply NEmpty_L. rewrite cardinal_Empty. eauto. }
+  assert (exists n, cardinal L = S n) as [n card_L].
+  { exists (cardinal L - 1). omega. }
+  assert (cardinal Sp = 0) as card_Sp.
+  { apply cardinal_Empty. assumption. }
+  subst Sp.
+  subst L.
+  induction s;
+    simpl;
+      rewrite card_L;
+      rewrite card_Sp;
+    simpl;
+    rewrite getAnn_setTopAnn;
+    rewrite card_L;
+      rewrite card_Sp;
+    simpl;
+      subst x;
+      subst L';
+      rewrite cardinal_tl with (n:=n);
+      eauto;
+    rewrite card_Sp;
+      simpl;
+    reflexivity.
+Qed.
